feat: prove that omega-regular languages are closed under left-concatenation by regular languages

Cslib/Foundations/Semantics/LTS/Basic.lean
@@ -127,6 +127,39 @@ theorem LTS.MTr.nil_eq (h : lts.MTr s1 [] s2) : s1 = s2 := by
   cases h
   rfl
 
+/-- A generalized `MTr` is a `MTr` augmented with intermediate states. -/
+@[scoped grind =]
+def LTS.GMTr (lts : LTS State Label)
+    (s1 : State) (μs : List Label) (ss : List State) (s2 : State) : Prop :=
+  ∃ _ : ss.length = μs.length + 1, ss[0] = s1 ∧ ss[μs.length] = s2 ∧
+    ∀ k, ∀ _ : k < μs.length, lts.Tr ss[k] μs[k] ss[k + 1]
+
+/-- Every `GMTr` can be projected onto a `MTr`. -/
+theorem LTS.GMTr.proj_MTr {lts : LTS State Label} {s1 s2 : State} {μs : List Label}
+    {ss : List State} (h : lts.GMTr s1 μs ss s2) : lts.MTr s1 μs s2 := by
+  obtain ⟨_, _, _, h_tr⟩ := h
+  have h_mtr (k) (h_k : k ≤ μs.length) : lts.MTr s1 (μs.take k) ss[k] := by
+    induction k
+    case zero => grind
+    case succ k h_ind =>
+      have := LTS.MTr.stepR lts (h_ind (by grind)) (h_tr k (by grind))
+      grind [List.take_append_getElem]
+  grind
+
+/-- Every `MTr` has a corresponding `GMTr` projecting onto it. -/
+theorem LTS.MTr.exists_GMTr {lts : LTS State Label} {s1 s2 : State} {μs : List Label}
+    (h : lts.MTr s1 μs s2) : ∃ ss, lts.GMTr s1 μs ss s2 := by
+  induction h
+  case refl t =>
+    use [t]
+    grind
+  case stepL t1 μ t2 μs t3 h_tr h_mtr h_ind =>
+    obtain ⟨ss', _, _, _, _⟩ := h_ind
+    use [t1] ++ ss'
+    refine ⟨by grind, by grind, by grind, ?_⟩
+    intro k
+    by_cases k = 0 <;> grind
+
 /-- A state `s1` can reach a state `s2` if there exists a multi-step transition from
 `s1` to `s2`. -/
 @[scoped grind =]
